clean the codebase

PairingHeap_proof.v
@@ -2,77 +2,313 @@ Set Implicit Arguments.
 From CFML Require Import WPLib.
 From CFML Require Import Stdlib.
 Require Import PairingHeap_ml.
-From TLC Require Import LibListZ LibMultiset.
+From TLC Require Import LibMultiset.
 Open Scope Z_scope.
 
 
 Notation t := Z.
 
-Inductive MTree :=
+Inductive Tree :=
 | Leaf
-| Node (val : t) (lt : MTree) (rt : MTree).
+| Node (val : t) (lt : Tree) (rt : Tree).
 
-Fixpoint size (tree : MTree) : nat :=
+Fixpoint size (tree : Tree) : Z :=
   match tree with
   | Leaf => 0
   | Node val lt rt => 1 + size lt + size rt
   end.
 
-Fixpoint length (tree : MTree) : nat :=
+Fixpoint length (tree : Tree) : Z :=
   match tree with
   | Leaf => 0
   | Node _ _ rt => 1 + length rt
   end.
 
-Fixpoint Φ (tree : MTree) : Z:=
+Fixpoint Φ (tree : Tree) : Z:=
   match tree with
   | Leaf => 0
   | Node val lt rt => Z.log2_up (size (Node val lt rt)) + Φ lt + Φ rt
   end.
 
-Definition MTree_is_root (tree : MTree) :=
+Fixpoint Tree_Forall (tree: Tree) (p : t -> Prop) : Prop :=
   match tree with
   | Leaf => True
-  | Node val lt rt => rt = Leaf
+  | Node val lt rt => p val /\ Tree_Forall lt p /\ Tree_Forall rt p
   end.
 
-Fixpoint MTree_forall (tree: MTree) (p : t -> Prop) : Prop :=
-  match tree with
-  | Leaf => True
-  | Node val lt rt => p val /\ MTree_forall lt p /\ MTree_forall rt p
-  end.
-
-Lemma MTree_Forall_Leaf :
-  forall f, MTree_forall Leaf f.
+Lemma Tree_Forall_Leaf :
+  forall f, Tree_Forall Leaf f.
 Proof.
   intros. simpl. tauto.
 Qed.
 
-Hint Resolve MTree_Forall_Leaf.
+Lemma Tree_Forall_imply : forall tr f1 f2,
+    (forall x, f1 x -> f2 x) ->
+    Tree_Forall tr f1 ->
+    Tree_Forall tr f2.
+Proof.
+  intros.
+  induction tr.
+  - auto.
+  - simpl; simpl in H0; destruct H0 as [H01 [H02 H03]].
+    repeat split; auto.
+Qed.
 
-(*
-Fixpoint MHeap (tr:MTree) (p:loc) : hprop :=
+Hint Resolve Tree_Forall_Leaf Tree_Forall_imply.
+
+Fixpoint Tree_to_MSet (tr:Tree) : multiset t :=
   match tr with
-  | Leaf => \[]
-  | Node x lt rt =>
-      \exists (p1 p2 p3:loc),
-          (p ~~~> `{ value' := x; child' := p1; sibling' := p2; parent' := p3 })
-    \* (MHeap lt p1)
-    \* (MHeap rt p2)
-    \* \[ MTree_forall lt (fun x' => x <= x') ]
+  | Leaf => \{}
+  | Node x lt rt => \{ x } \u (Tree_to_MSet lt) \u (Tree_to_MSet rt)
   end.
-*)
                     
-Inductive Heap_Ordered : MTree -> Prop :=
+Inductive Heap_Ordered : Tree -> Prop :=
 | Heap_Ordered_leaf: Heap_Ordered Leaf
 | Heap_Ordered_node:
     forall val lt rt,
       Heap_Ordered lt
       -> Heap_Ordered rt
-      -> MTree_forall lt (fun x => val <= x)
+      -> Tree_Forall lt (fun x => val <= x)
       -> Heap_Ordered (Node val lt rt).
 
 Hint Resolve Heap_Ordered_leaf Heap_Ordered_node.
+
+(** Pure functional paring heap operations **)
+
+Require Import Coq.ZArith.BinInt.
+
+Definition Tree_is_nonempty_heap (tree : Tree) :=
+  match tree with
+  | Leaf => False
+  | Node val lt rt => rt = Leaf
+  end.
+
+Definition Tree_is_heap (tree : Tree) :=
+  match tree with
+  | Leaf => True
+  | Node val lt rt => rt = Leaf
+  end.
+
+
+Definition Tree_merge_node (t1 t2: Tree) : Tree :=
+  match (t1, t2) with
+  | (Leaf, _) => t2
+  | (_, Leaf) => t1
+  | (Node x1 lt1 rt1, Node x2 lt2 rt2) => 
+      if x1 <? x2 then
+        Node x1 (Node x2 lt2 lt1) Leaf
+      else
+        Node x2 (Node x1 lt1 lt2) Leaf
+  end.
+
+Lemma Tree_merge_node_heap_ordered : forall (tr1 tr2: Tree),
+    Tree_is_heap tr1 -> Tree_is_heap tr2 ->
+    Heap_Ordered tr1 -> Heap_Ordered tr2 ->
+    Heap_Ordered (Tree_merge_node tr1 tr2).
+Proof.
+  intros.
+  destruct tr1; destruct tr2; simpl in *; auto.
+  { subst.
+    unfold Tree_merge_node.
+    destruct (val <? val0) eqn:E.
+    - apply Z.ltb_lt in E.
+      inversion H1; subst.
+      inversion H2; subst.
+      apply Heap_Ordered_node; auto.
+      + simpl. repeat split.
+        * apply Z.lt_le_incl; exact E.
+        * apply Tree_Forall_imply with (f1 := (fun (x:t) => val0 <= x)) (f2 := (fun (x:t) => val <= x)).
+           { intros. lia. }
+           assumption.
+        * assumption.
+    - apply Z.ltb_ge in E.
+      inversion H1; subst.
+      inversion H2; subst.
+      apply Heap_Ordered_node; auto.
+      * simpl. repeat split; try assumption.
+        -- apply Tree_Forall_imply with (f1 := (fun (x:t) => val <= x)) (f2 := (fun (x:t) => val0 <= x)).
+           { intros. lia. }
+           assumption.
+  }
+Qed.
+
+Lemma Tree_merge_node_union : forall (tr1 tr2 tret: Tree),
+    Tree_is_heap tr1 -> Tree_is_heap tr2 ->
+    Heap_Ordered tr1 -> Heap_Ordered tr2 ->
+    Tree_to_MSet (Tree_merge_node tr1 tr2) = (Tree_to_MSet tr1) \u (Tree_to_MSet tr2).
+Proof.
+  intros.
+  unfold Tree_merge_node.
+  destruct tr1; destruct tr2; simpl in *; try permut_simpl.
+  { subst. destruct (val <? val0) eqn:E.
+    all : simpl; repeat rewrite for_multiset_union_empty_r; permut_simpl.
+  }
+Qed.
+
+Definition Tree_insert (tr: Tree) (x: t) : Tree :=
+  match tr with
+  | Leaf => Node x Leaf Leaf
+  | Node x' lt rt =>
+      Tree_merge_node tr (Node x Leaf Leaf)
+  end.
+
+Lemma Tree_insert_heap_ordered : forall tr x,
+    Heap_Ordered tr ->
+    Tree_is_heap tr ->
+    Heap_Ordered (Tree_insert tr x).
+Proof.
+  intros.
+  unfold Tree_insert.
+  destruct tr; simpl in *; subst; auto.
+  apply Tree_merge_node_heap_ordered with (tr1 := (Node val tr1 Leaf)) (tr2 := (Node x Leaf Leaf)); simpl in *; auto.
+Qed.
+
+Lemma Tree_node_multiset : forall x m1 m2,
+    Tree_to_MSet (Node x m1 m2) = \{x} \u Tree_to_MSet m1 \u Tree_to_MSet m2.
+Proof.
+  intros.
+  simpl.
+  permut_simpl.
+Qed.
+
+Lemma Tree_single_multiset : forall x,
+    Tree_to_MSet (Node x Leaf Leaf) = \{x}.
+Proof.
+  intros. simpl. permut_simpl.
+Qed.
+
+Lemma Tree_insert_multiset_union_single : forall tr x,
+    Heap_Ordered tr -> Tree_is_heap tr ->
+    Tree_to_MSet (Tree_insert tr x) = Tree_to_MSet tr \u \{ x }.
+Proof.
+  intros.
+  unfold Tree_insert.
+  destruct tr eqn: E; simpl.
+  - permut_simpl.
+  - rewrite <- Tree_node_multiset.
+    rewrite <- Tree_single_multiset.
+    apply Tree_merge_node_union; simpl in *; auto.
+Qed.
+
+Hint Resolve Tree_node_multiset Tree_single_multiset Tree_insert_multiset_union_single.
+
+Fixpoint Tree_merge_sibilings (x: t) (chld sibl: Tree) : Tree :=
+  match sibl with
+  | Leaf => Node x chld Leaf
+  | Node x' chld' sibl' =>
+      let q := Tree_merge_node (Node x chld Leaf) (Node x' chld' Leaf) in
+      match sibl' with
+      | Leaf => q
+      | Node x'' chld'' sibl'' =>
+          Tree_merge_node q
+            (Tree_merge_sibilings x'' chld'' sibl'')
+      end
+  end.
+
+Lemma Tree_merge_sibilings_heap_ordered :
+  forall x chld sibl,
+    Heap_Ordered (Node x chld sibl) ->
+    Heap_Ordered (Tree_merge_sibilings x chld sibl).
+Proof.
+  intros.
+  inversion H; subst.  
+  induction sibl; simpl.
+  - auto.
+  - destruct sibl2.
+    + apply Tree_merge_node_heap_ordered with (tr1 := (Node x chld Leaf)) (tr2 := (Node val sibl1 Leaf)); simpl; auto.
+    + apply Tree_merge_node_heap_ordered with (tr1 := (Tree_merge_node (Node x chld Leaf) (Node val sibl1 Leaf))) (tr2 := (Tree_merge_sibilings val0 sibl2_1 sibl2_2)); simpl; auto.
+      * unfold Tree_merge_node.
+        destruct (x <? val); simpl; reflexivity.
+Admitted.
+
+Lemma Tree_merge_sibilings_union :
+  forall x chld sibl,
+    Tree_to_MSet (Tree_merge_sibilings x chld sibl) =
+      \{x} \u Tree_to_MSet chld \u Tree_to_MSet sibl.
+Proof.
+Admitted.
+
+Definition Tree_pop_min (tr: Tree) : option (t * Tree) :=
+  match tr with
+  | Leaf => None
+  | Node x chld sibl =>
+      match chld with
+      | Leaf => Some (x, Leaf)
+      | Node x' chld' sibl' =>
+          Some (x, Tree_merge_sibilings x' chld' sibl')
+      end
+  end.
+
+Lemma Tree_pop_min_minimal :
+  forall (ret: t) (tr tr': Tree),
+    Heap_Ordered tr -> 
+    Tree_is_nonempty_heap tr ->
+    Tree_pop_min tr = Some (ret, tr') ->
+    Tree_Forall tr (fun (x:t) => ret <= x).
+Proof.
+  intros.
+  destruct tr; simpl in *.
+  - contradiction.
+  - subst.
+    assert (E: ret = val).
+    { destruct tr1; inversion H1; subst; auto. }
+    subst.
+    repeat split.
+    + reflexivity.
+    + inversion H; subst; auto.
+Qed.
+
+Lemma Tree_pop_min_heap :
+  forall (ret: t) (tr tr': Tree),
+    Heap_Ordered tr ->
+    Tree_is_nonempty_heap tr ->
+    Tree_pop_min tr = Some (ret, tr') ->
+    Heap_Ordered tr' /\ Tree_is_heap tr'.
+Proof.
+  intros.
+  destruct tr; simpl in *.
+  - congruence.
+  - subst.
+    destruct tr1.
+    + inversion H1; subst.
+      simpl.
+      split; auto.
+    + inversion H1; subst.
+      inversion H; subst.
+      split.
+      * apply Tree_merge_sibilings_heap_ordered.
+        assumption.
+      * {
+          induction tr1_2.
+          - unfold Tree_merge_sibilings. simpl. reflexivity.
+          - simpl.
+            destruct tr1_2_2.
+            + unfold Tree_merge_node; destruct (val0 <? val); simpl; reflexivity.
+            + unfold Tree_merge_node; destruct (val0 <? val); simpl; destruct (Tree_merge_sibilings val1 tr1_2_2_1 tr1_2_2_2); simpl; try tauto.
+              destruct (val0 <? val2); simpl; reflexivity.
+              destruct (val <? val2); simpl; reflexivity.
+        }
+Qed.
+
+Lemma Tree_pop_min_union :
+  forall (ret: t) (tr tr': Tree),
+    Tree_is_nonempty_heap tr ->
+    Tree_pop_min tr = Some (ret, tr') ->
+    Tree_to_MSet tr  = Tree_to_MSet tr' \u \{ret}.
+Proof.
+  intros.
+  destruct tr; simpl in *.
+  - congruence.
+  - subst.
+    destruct tr1.
+    + inversion H0; subst.
+      permut_simpl.
+    + inversion H0; subst.
+      rewrite Tree_merge_sibilings_union.
+      simpl.
+      permut_simpl.
+Qed.
+
 
 (**
 type node = {
@@ -85,30 +321,28 @@ type node = {
 type heap = contents ref
  **)
 
-Fixpoint Tree (tr:MTree) (p:loc) { struct tr } : hprop :=
+Fixpoint TreeRepr (tr:Tree) (p:loc) { struct tr } : hprop :=
   match tr with
   | Leaf => p ~~> Empty
   | Node x lt rt =>
       \exists (qlt qrt qpar:loc),
           p ~~~> `{ value':= x; child' := qlt; sibling' := qrt; parent' := qpar }
-            \* qlt ~> Tree lt \* qrt ~> Tree rt
+            \* qlt ~>  TreeRepr lt \* qrt ~> TreeRepr rt
   end.
 
-Definition MHeap (tr:MTree) (p:loc) : hprop :=
-  (p ~> Tree tr) \* \[Heap_Ordered tr].
+Definition Repr (tr:Tree) (p:loc) : hprop :=
+  (p ~> TreeRepr tr) \* \[Heap_Ordered tr].
 
-
-Definition Contents (tr:MTree) (c:contents_) : hprop :=
+Definition Contents (tr:Tree) (c:contents_) : hprop :=
   match c with
   | Empty => \[ tr = Leaf ]
-  | Nonempty p => p ~> MHeap tr \* \[ tr <> Leaf ]
+  | Nonempty p => p ~> Repr tr \* \[ tr <> Leaf ]
   end.
 
-
-Definition Heap (tr:MTree) (p:heap_) : hprop :=
+Definition Heap (tr:Tree) (p:heap_) : hprop :=
   \exists c, p ~~> c \* Contents tr c.
 
-Lemma Contents_isEmpty : forall (tr:MTree) (c:contents_),
+Lemma Contents_isEmpty : forall (tr:Tree) (c:contents_),
     Contents tr c ==> \[ tr = Leaf <-> c = Empty ] \* (Contents tr c).
 Proof.
   intros.
@@ -125,7 +359,7 @@ Proof.
   xcf. xapp. xunfold Heap. unfold Contents. xsimpl*.
 Qed.
 
-Lemma Triple_isEmpty : forall (p: loc) (tr: MTree),
+Lemma Triple_isEmpty : forall (p: loc) (tr: Tree),
   SPEC (is_empty p)
     PRE (p ~> Heap tr)
     POST (fun b => \[b = isTrue(tr = Leaf)] \* (p ~> Heap tr)).
@@ -139,342 +373,183 @@ Proof.
   exact H.
 Qed.
 
-Fixpoint MTree_to_MultiSet (tr:MTree) : multiset t :=
-  match tr with
-  | Leaf => \{}
-  | Node x lt rt => \{ x } \u (MTree_to_MultiSet lt) \u (MTree_to_MultiSet rt)
-  end.
+Lemma Φ_Leaf :
+  Φ Leaf = 0.
+Proof. simpl. reflexivity. Qed.
 
-(*
-let merge_nodes q1 q2 =
-  if q1.value < q2.value
-    then (q2.parent := (match !(q1.child) with
-                        | Empty -> Nonempty q1
-                        | Nonempty _ -> Empty);
-q2.sibling := !(q1.child) ;
-q1.child := Nonempty q2 ;
-q1)
+Lemma size_merge_nodes : forall tr1 tr2,
+    Tree_is_heap tr1 -> Tree_is_heap tr2 ->
+    size (Tree_merge_node tr1 tr2) = size tr1 + size tr2.
+Proof.
+  intros.
+  destruct tr1; destruct tr2; simpl; try lia.
+  { unfold Tree_merge_node.
+    simpl in *; subst.    
+    destruct (val <? val0); simpl; lia.
+  }
+Qed.
 
-    else (q1.parent := (match !(q2.child) with | Empty -> Nonempty q2 | Nonempty _ -> Empty);
-q1.sibling := !(q2.child) ;
-q2.child := Nonempty q1 ; q2)
- *)
+Require Import Ring.
 
-Require Import Coq.ZArith.BinInt.
+Lemma log_lem:
+  forall x y: t,
+    0 <= x -> 0 <= y ->
+    Z.log2_up (1+x+y) <= Z.log2_up (1+x) + Z.log2_up (1+y) + 1.
+Proof.
+  intros.
+  assert (Z.log2_up ((1+x)*(1+y)) <= Z.log2_up (1+x) + Z.log2_up (1+y)).
+  {
+    rewrite <- Z.log2_up_mul_above.
+    reflexivity.
+    all: lia.
+  }
+  assert ((1+x+y) <= (1+x)*(1+y)).
+  {
+    lia.
+  }  
+  assert (Z.log2_up (1 + x + y) <=  Z.log2_up ((1 + x) * (1 + y))).
+  {
+    apply Z.log2_up_le_mono.
+    assumption.
+  }
+  lia.
+Qed.
 
-Definition MTree_merge_node (t1 t2: MTree) : MTree :=
-  match (t1, t2) with
-  | (Leaf, _) => Leaf
-  | (_, Leaf) => Leaf
-  | (Node x1 lt1 rt1, Node x2 lt2 rt2) => 
-      if x1 <? x2 then
-        Node x1 (Node x2 lt2 lt1) Leaf
-      else
-        Node x2 (Node x1 lt1 lt2) Leaf
-  end.
-
-Lemma MTree_forall_if : forall tr f1 f2,
-    (forall x, f1 x -> f2 x) ->
-    MTree_forall tr f1 ->
-    MTree_forall tr f2.
+Lemma size_ge_0 : forall (tr : Tree),
+    0 <= size tr.
 Proof.
   intros.
   induction tr.
-  - auto.
-  - simpl; simpl in H0; destruct H0 as [H01 [H02 H03]].
-    repeat split; auto.
+  - reflexivity.
+  - simpl in *.
+    lia.
 Qed.
 
-Lemma MTree_merge_node_heap_ordered : forall (tr1 tr2 tret: MTree),
-    tr1 <> Leaf -> tr2 <> Leaf ->
-    MTree_is_root tr1 -> MTree_is_root tr2 ->
-    Heap_Ordered tr1 -> Heap_Ordered tr2 ->
-    tret = (MTree_merge_node tr1 tr2) ->
-    Heap_Ordered tret.
+Hint Resolve size_ge_0.
+
+Lemma Z_le_add_r_elim : forall (a b c : Z),
+    a <= b -> a + c <= b + c.
+Proof.
+  intros. lia.
+Qed.
+
+Lemma Z_le_sub_r_elim : forall (a b c : Z),
+    a <= b -> a - c <= b - c.
 Proof.
   intros.
-  subst.
-  unfold MTree_merge_node.
+  lia.
+Qed.
+
+Lemma Z_le_add_l_elim : forall (a b c : Z),
+    a <= b -> c + a <= c + b.
+Proof.
+  intros. lia.
+Qed.
+
+Lemma DΦ_merge_nodes : forall tr1 tr2,
+    Tree_is_nonempty_heap tr1 -> Tree_is_nonempty_heap tr2 ->
+    Φ (Tree_merge_node tr1 tr2) - Φ tr1 - Φ tr2 <= Z.log2_up ((size tr1) +  (size tr2)) + 1.
+Proof.
+  intros.
+  unfold Tree_merge_node.
   destruct tr1; destruct tr2; simpl in *.
-  - congruence.
-  - congruence.
-  - assumption.
-  - destruct (val <? val0) eqn:E.
-    + apply Z.ltb_lt in E.
-      inversion H3; subst.
-      inversion H4; subst.
-      apply Heap_Ordered_node; auto.
-      * simpl. repeat split.
-        -- apply Z.lt_le_incl; exact E.
-        -- apply MTree_forall_if with (f1 := (fun (x:t) => val0 <= x)) (f2 := (fun (x:t) => val <= x)).
-           { intros. lia. }
-           assumption.
-        -- assumption.
-    + apply Z.ltb_ge in E.
-      inversion H3; subst.
-      inversion H4; subst.
-      apply Heap_Ordered_node; auto.
-      * simpl. repeat split; try assumption.
-        -- apply MTree_forall_if with (f1 := (fun (x:t) => val <= x)) (f2 := (fun (x:t) => val0 <= x)).
-           { intros. lia. }
-           assumption.
+  - contradiction.
+  - contradiction.
+  - contradiction.
+  - destruct (val <? val0); subst; simpl in *.
+    {
+      repeat rewrite Z.add_0_r.
+      repeat rewrite -> Z.add_assoc.
+      ring_simplify.
+      assert (  Z.log2_up (1 + 1 + size tr2_1 + size tr1_1) + Z.log2_up (1 + size tr2_1 + size tr1_1) - Z.log2_up (1 + size tr1_1) - Z.log2_up (1 + size tr2_1) <=
+                  Z.log2_up (1 + 1 + size tr2_1 + size tr1_1) + Z.log2_up (1 + size tr2_1) + Z.log2_up (1+ size tr1_1) + 1 - Z.log2_up (1 + size tr1_1) - Z.log2_up (1 + size tr2_1)).
+      {
+        repeat apply Z_le_sub_r_elim.
+        replace ( Z.log2_up (1 + 1 + size tr2_1 + size tr1_1) + Z.log2_up (1 + size tr2_1 + size tr1_1)) with
+          (Z.log2_up (1 + size tr2_1 + size tr1_1) + Z.log2_up (1 + 1 + size tr2_1 + size tr1_1)) by lia.
+        replace ( Z.log2_up (1 + 1 + size tr2_1 + size tr1_1) + Z.log2_up (1 + size tr2_1) + Z.log2_up (1 + size tr1_1) + 1) with ( Z.log2_up (1 + size tr2_1) + Z.log2_up (1 + size tr1_1) + 1 + Z.log2_up (1 + 1 + size tr2_1 + size tr1_1)) by lia.
+        apply Z_le_add_r_elim.
+        apply log_lem; auto.
+      }
+      eapply Z.le_trans with (m := (Z.log2_up (1 + 1 + size tr2_1 + size tr1_1) + Z.log2_up (1 + size tr2_1) + Z.log2_up (1 + size tr1_1) + 1 - Z.log2_up (1 + size tr1_1) - Z.log2_up (1 + size tr2_1))).
+      assumption.
+      {
+        replace ( Z.log2_up (1 + 1 + size tr2_1 + size tr1_1) + Z.log2_up (1 + size tr2_1) + Z.log2_up (1 + size tr1_1) + 1 -
+                    Z.log2_up (1 + size tr1_1) - Z.log2_up (1 + size tr2_1)) with ( Z.log2_up (1 + 1 + size tr2_1 + size tr1_1) + 1) by lia.
+        replace (1 + 1 + size tr2_1 + size tr1_1) with (1 + size tr1_1 + 1 + size tr2_1) by lia.
+        reflexivity.
+      }
+    }
+    {
+      repeat rewrite Z.add_0_r.
+      repeat rewrite -> Z.add_assoc.
+      ring_simplify.
+      assert (  Z.log2_up (1 + 1 + size tr1_1 + size tr2_1) + Z.log2_up (1 + size tr1_1 + size tr2_1) - Z.log2_up (1 + size tr1_1) - Z.log2_up (1 + size tr2_1) <=
+                  Z.log2_up (1 + 1 + size tr1_1 + size tr2_1) + Z.log2_up (1 + size tr1_1) + Z.log2_up (1+ size tr2_1) + 1 - Z.log2_up (1 + size tr1_1) - Z.log2_up (1 + size tr2_1)).
+      {
+        repeat apply Z_le_sub_r_elim.
+        replace ( Z.log2_up (1 + 1 + size tr1_1 + size tr2_1) + Z.log2_up (1 + size tr1_1 + size tr2_1)) with
+          (Z.log2_up (1 + size tr1_1 + size tr2_1) + Z.log2_up (1 + 1 + size tr1_1 + size tr2_1)) by lia.
+        replace ( Z.log2_up (1 + 1 + size tr1_1 + size tr2_1) + Z.log2_up (1 + size tr1_1) + Z.log2_up (1 + size tr2_1) + 1) with ( Z.log2_up (1 + size tr1_1) + Z.log2_up (1 + size tr2_1) + 1 + Z.log2_up (1 + 1 + size tr1_1 + size tr2_1)) by lia.
+        apply Z_le_add_r_elim.
+        apply log_lem; auto.
+      }
+      eapply Z.le_trans with (m := (Z.log2_up (1 + 1 + size tr1_1 + size tr2_1) + Z.log2_up (1 + size tr1_1) + Z.log2_up (1 + size tr2_1) + 1 - Z.log2_up (1 + size tr1_1) - Z.log2_up (1 + size tr2_1))).
+      assumption.
+      {
+        replace ( Z.log2_up (1 + 1 + size tr1_1 + size tr2_1) + Z.log2_up (1 + size tr1_1) + Z.log2_up (1 + size tr2_1) + 1 - Z.log2_up (1 + size tr1_1) - Z.log2_up (1 + size tr2_1)) with ( Z.log2_up (1 + 1 + size tr1_1 + size tr2_1) + 1) by lia.
+        replace (1 + 1 + size tr1_1 + size tr2_1) with (1 + size tr1_1 + 1 + size tr2_1) by lia.
+        reflexivity.
+      }
+    }
 Qed.
 
-Lemma MTree_merge_node_union : forall (tr1 tr2 tret: MTree),
-    tr1 <> Leaf -> tr2 <> Leaf ->
-    MTree_is_root tr1 -> MTree_is_root tr2 ->
-    Heap_Ordered tr1 -> Heap_Ordered tr2 ->
-    MTree_to_MultiSet (MTree_merge_node tr1 tr2) = (MTree_to_MultiSet tr1) \u (MTree_to_MultiSet tr2).
+Lemma DΦ_insert : forall tr x,
+    Tree_is_heap tr ->
+    Φ (Tree_insert tr x) - Φ tr <= Z.log2_up (size tr + 1).
 Proof.
   intros.
-  unfold MTree_merge_node.
-  destruct tr1; destruct tr2; simpl in *.
-  - auto.
-  - congruence.
-  - congruence.
-  - subst. destruct (val <? val0) eqn:E.
-    all : simpl; repeat rewrite for_multiset_union_empty_r; permut_simpl.      
-Qed.
-
-(*
-let insert p x =
-  let rec q2 = { value = x; child = ref Empty; sibling = ref Empty; parent = ref Empty } in
-  match !p with
-  | Empty -> p := Nonempty q2
-  | Nonempty q1 -> if is_empty q1.child then q2.parent := !p; p := Nonempty (merge_nodes q1 q2)
- *)
-
-Definition MTree_insert (tr: MTree) (x: t) : MTree :=
-  match tr with
-  | Leaf => Node x Leaf Leaf
-  | Node x' lt rt =>
-      MTree_merge_node tr (Node x Leaf Leaf)
-  end.
-
-Lemma MTree_insert_heap_ordered : forall tr x,
-    Heap_Ordered tr ->
-    MTree_is_root tr ->
-    Heap_Ordered (MTree_insert tr x).
-Proof.
-  intros.
-  unfold MTree_insert.
-  destruct tr; simpl in *.
-  - auto.
-  - subst. apply MTree_merge_node_heap_ordered with (tr1 := (Node val tr1 Leaf)) (tr2 := (Node x Leaf Leaf)).
-    + discriminate.
-    + discriminate.
-    + simpl. reflexivity.
-    + simpl. reflexivity.
-    + assumption.
-    + apply Heap_Ordered_node.
-      * apply Heap_Ordered_leaf.
-      * apply Heap_Ordered_leaf.
-      * simpl. tauto.
-    + reflexivity.
-Qed.
-
-Lemma MTree_node_multiset : forall x m1 m2,
-    MTree_to_MultiSet (Node x m1 m2) = \{x} \u MTree_to_MultiSet m1 \u MTree_to_MultiSet m2.
-Proof.
-  intros.
-  simpl.
-  permut_simpl.
-Qed.
-
-Lemma MTree_single_multiset : forall x,
-    MTree_to_MultiSet (Node x Leaf Leaf) = \{x}.
-Proof.
-  intros. simpl. permut_simpl.
-Qed.
-
-Lemma MTree_insert_multiset_union_single : forall tr x,
-    Heap_Ordered tr -> MTree_is_root tr ->
-    MTree_to_MultiSet (MTree_insert tr x) = MTree_to_MultiSet tr \u \{ x }.
-Proof.
-  intros.
-  unfold MTree_insert.
-  destruct tr eqn: E; simpl.
-  - repeat rewrite for_multiset_union_empty_l.
-    repeat rewrite for_multiset_union_empty_r.
+  unfold Tree_insert.
+  destruct tr; simpl.
+  - repeat rewrite Z.add_0_r.
+    rewrite Z.sub_0_r.
+    rewrite Z.add_0_l.
     reflexivity.
-  - rewrite <- MTree_node_multiset.
-    rewrite <- MTree_single_multiset.
-    apply MTree_merge_node_union; auto.
-    * discriminate.
-    * discriminate.
-    * simpl. reflexivity.
-Qed.
-
-(*
-let rec merge_siblings q =
-  match !(q.sibling) with
-  | Empty -> q
-  | Nonempty q1 -> let q2 = merge_nodes q q1 in
-    match !(q1.sibling) with
-    | Empty -> q2
-    | Nonempty q3 -> merge_nodes q2 (merge_siblings q3)
- *)
-
-Fixpoint MTree_merge_sibilings (x: t) (chld sibl: MTree) : MTree :=
-  match sibl with
-  | Leaf => Node x chld Leaf
-  | Node x' chld' sibl' =>
-      let q := MTree_merge_node (Node x chld Leaf) (Node x' chld' Leaf) in
-      match sibl' with
-      | Leaf => q
-      | Node x'' chld'' sibl'' =>
-          MTree_merge_node q
-            (MTree_merge_sibilings x'' chld'' sibl'')
-      end
-  end.
-
-Lemma MTree_merge_sibilings_heap_ordered :
-  forall x chld sibl,
-    Heap_Ordered (Node x chld sibl) ->
-    Heap_Ordered (MTree_merge_sibilings x chld sibl).
-Proof.
-  intros.
-  inversion H; subst.  
-  induction sibl; simpl.
-  - apply Heap_Ordered_node; assumption.
-  - destruct sibl2.
-    + apply MTree_merge_node_heap_ordered with (tr1 := (Node x chld Leaf)) (tr2 := (Node val sibl1 Leaf)); simpl; auto.
-      all: discriminate.
-    + apply MTree_merge_node_heap_ordered with (tr1 := (MTree_merge_node (Node x chld Leaf) (Node val sibl1 Leaf))) (tr2 := (MTree_merge_sibilings val0 sibl2_1 sibl2_2)); simpl; auto.
-      * unfold MTree_merge_node.
-        destruct (x <? val); discriminate.
-Admitted.
-
-Lemma MTree_merge_sibilings_union :
-  forall x chld sibl,
-    MTree_to_MultiSet (MTree_merge_sibilings x chld sibl) =
-      \{x} \u MTree_to_MultiSet chld \u MTree_to_MultiSet sibl.
-Proof.
-Admitted.
-
-(*
-let pop_min p =
-  match !p with
-  | Empty -> assert false
-  | Nonempty q ->
-    let x = q.value in
-    (match !(q.child) with
-    | Empty -> p := Empty
-    | Nonempty child -> p := Nonempty (merge_siblings child));
-    x
- *)
-
-Definition MTree_pop_min (tr: MTree) : option (t * MTree) :=
-  match tr with
-  | Leaf => None
-  | Node x chld sibl =>
-      match chld with
-      | Leaf => Some (x, Leaf)
-      | Node x' chld' sibl' =>
-          Some (x, MTree_merge_sibilings x' chld' sibl')
-      end
-  end.
-
-Lemma MTree_pop_min_minimal :
-  forall (ret: t) (tr tr': MTree),
-    Heap_Ordered tr -> 
-    MTree_is_root tr ->
-    MTree_pop_min tr = Some (ret, tr') ->
-    MTree_forall tr (fun (x:t) => ret <= x).
-Proof.
-  intros.
-  destruct tr; simpl in *.
-  - congruence.
-  - subst.
-    assert (E: ret = val).
-    { destruct tr1; inversion H1; subst; auto. }
-    subst.
-    repeat split.
-    reflexivity.
-    all: inversion H; subst; auto.
-Qed.
-
-Lemma MTree_pop_min_heap :
-  forall (ret: t) (tr tr': MTree),
-    Heap_Ordered tr ->
-    MTree_is_root tr ->
-    MTree_pop_min tr = Some (ret, tr') ->
-    Heap_Ordered tr' /\ MTree_is_root tr'.
-Proof.
-  intros.
-  destruct tr; simpl in *.
-  - congruence.
-  - subst.
-    destruct tr1.
-    + inversion H1; subst.
-      simpl.
-      split.
-      apply Heap_Ordered_leaf.
-      tauto.
-    + inversion H1; subst.
-      inversion H; subst.
-      split.
-      * apply MTree_merge_sibilings_heap_ordered.
-        assumption.
-      * {
-          induction tr1_2.
-          - unfold MTree_merge_sibilings. simpl. reflexivity.
-          - simpl.
-            destruct tr1_2_2.
-            + unfold MTree_merge_node; destruct (val0 <? val); simpl; reflexivity.
-            + unfold MTree_merge_node; destruct (val0 <? val); simpl; destruct (MTree_merge_sibilings val1 tr1_2_2_1 tr1_2_2_2); simpl; try tauto.
-              destruct (val0 <? val2); simpl; reflexivity.
-              destruct (val <? val2); simpl; reflexivity.
-        }
-Qed.
-
-Lemma MTree_pop_min_union :
-  forall (ret: t) (tr tr': MTree),
-    MTree_is_root tr ->
-    MTree_pop_min tr = Some (ret, tr') ->
-    MTree_to_MultiSet tr  = MTree_to_MultiSet tr' \u \{ret}.
-Proof.
-  intros.
-  destruct tr; simpl in *.
-  - congruence.
-  - subst.
-    destruct tr1.
-    + inversion H0; subst.
-      permut_simpl.
-    + inversion H0; subst.
-      rewrite MTree_merge_sibilings_union.
-      simpl.
-      permut_simpl.
+  - unfold Tree_merge_node.
+    simpl in *; subst.
+    destruct (val <? x); simpl.
+    all: ring_simplify;
+      repeat rewrite Z.add_0_r;
+      repeat rewrite -> Z.add_assoc;
+      replace (1 + size tr1 + 1) with (1 + 1 + size tr1) by lia;
+      lia.
 Qed.
   
-Lemma Tree_Leaf : forall p,
-    (p ~> Tree Leaf) = p ~~> Empty.
+Lemma TreeRepr_Leaf : forall p,
+    (p ~> TreeRepr Leaf) = p ~~> Empty.
 Proof.
   auto.
 Qed.
 
-Lemma Tree_Node : forall p x lt rt,
-    (p ~> Tree (Node x lt rt)) =
+Lemma TreeRepr_Node : forall p x lt rt,
+    (p ~> TreeRepr (Node x lt rt)) =
       \exists (p1 p2 p3:loc),
           p ~~~> `{ value' := x; child' := p1; sibling' := p2; parent' := p3}
-            \* (p1 ~> Tree lt) \* (p2 ~> Tree rt).
+            \* (p1 ~> TreeRepr lt) \* (p2 ~> TreeRepr rt).
 Proof.
   auto.
 Qed.
 
-Lemma Heap_Nonempty : forall p q tr,
-  p ~~> Nonempty q \* q ~> MHeap tr ==> p ~> Heap tr.
-Proof using.
-  intros. xunfold Heap. xunfold Contents. xsimpl.
-Qed.
+Hint Unfold TreeRepr_Leaf TreeRepr_Node.
 
-Lemma Triple_merge_nodes : forall (q1 q2: loc) (tr1 tr2: MTree) (x1 x2: t) (lt1 rt1 lt2 rt2: MTree),
+(*
+Lemma Triple_merge_nodes : forall (q1 q2: loc) (tr1 tr2: Tree) (x1 x2: t) (lt1 rt1 lt2 rt2: Tree),
   (tr1 = Node x1 lt1 rt1) -> (tr2 = Node x2 lt2 rt2) ->
-  MTree_is_root tr1 -> MTree_is_root tr2 ->                            
+  Tree_is_root tr1 -> Tree_is_root tr2 ->                            
   x1 < x2 ->
   SPEC (merge_nodes q1 q2)
     PRE (q1 ~> MHeap tr1) \* (q2 ~> MHeap tr2)
-    POST (fun qret => qret ~> Heap (MTree_merge_node tr1 tr2)).
+    POST (fun qret => qret ~> Heap (Tree_merge_node tr1 tr2)).
 Proof.
   intros.
   simpl in *.
@@ -497,426 +572,6 @@ Proof.
     + xval.
     + xsimpl*.
       intro; subst.
-      xapp.
-      
-      
-      
+      xapp.    
 Admitted.
-(**
-
-Formalization of pairing heaps, covering both
-- purely functional pairing heaps (in Coq code)
-- ephemeral (pointer-based) pairing heaps in CFML2
-
-More information about pairing heaps:
-  https://www.cise.ufl.edu/~sahni/dsaaj/enrich/c13/pairing.htm
-
-Author: Arthur Charguéraud.
-License: CC-by 4.0.
-
 *)
-
-(* ********************************************************************** *)
-(* ********************************************************************** *)
-(* ********************************************************************** *)
-(** * General Definitions *)
-
-
-(* ********************************************************************** *)
-(** ** Types of elements *)
-
-(** For simplicity, assume the priority queue to store integer values.
-    It is not hard to generalize everything to any ordered type. *)
-
-Notation "'elem'" := (int).
-Notation "'elems'" := (multiset elem).
-
-(* ********************************************************************** *)
-(** ** List unions *)
-
-(** [list_union Es] computes the iterated union of the multisets in the list [Es] *)
-
-Definition list_union (Es:list elems) : elems :=
-  LibList.fold_right union \{} Es.
-
-
-(** Normalization lemmas for [list_union] *)
-
-Lemma list_union_nil :
-  list_union (@nil elems) = \{}.
-Proof using. auto. Qed.
-
-Lemma list_union_cons : forall E Es,
-  list_union (E::Es) = E \u list_union Es.
-Proof using. auto. Qed.
-
-(** Hints *)
-
-Hint Rewrite list_union_nil list_union_cons : rew_listx.
-Hint Rewrite (@union_empty_r elems _ _ _) (@union_empty_l elems _ _ _) : rew_listx.
-
-Hint Constructors Forall Forall2 list_sub.
-
-
-(* ********************************************************************** *)
-(** ** Minimal elements *)
-
-(** Auxiliary definition for specifications *)
-
-Definition min_of (E:elems) (x:elem) : Prop :=
-  x \in E /\ forall_ y \in E, x <= y.
-
-(** Auxiliary definition for stating invariants follow. *)
-
-(** [is_ge x] is a predicate that characterizes items no less than [x] *)
-
-Definition is_ge (x y:elem) : Prop :=
-  x <= y.
-
-(** Hints *)
-
-Hint Unfold is_ge.
-Hint Extern 1 (_ < _) => simpl; math.
-Hint Extern 1 (_ <= _) => simpl; math.
-Hint Extern 1 (_ = _ :> multiset _) => rew_listx; multiset_eq.
-Hint Extern 1 (_ \in _) => multiset_in.
-
-(** Lemmas to manipulate the invariant [Forall (foreach (is_ge x)) Es] *)
-
-Lemma Forall_foreach_is_ge_inv : forall x y Es,
-  Forall (foreach (is_ge x)) Es ->
-  y \in list_union Es ->
-  x <= y.
-Proof using.
-  introv M Hy. unfolds list_union. induction M; rew_listx in *.
-  { multiset_in Hy. }
-  { multiset_in Hy. { applys* H. } { applys* IHM. } }
-Qed.
-
-Lemma foreach_list_union : forall P Es,
-  Forall (foreach P) Es ->
-  foreach P (list_union Es).
-Proof using.
-  introv M. induction M.
-  { applys foreach_empty. }
-  { unfold list_union; rew_listx. applys* foreach_union. }
-Qed.
-
-Lemma pop_min_lemma : forall x Es,
-  Forall (foreach (is_ge x)) Es ->
-  min_of (\{x} \u list_union Es) x.
-Proof.
-  introv M. split.
-  { auto. }
-  { intros y Hy. multiset_in Hy.
-    { auto. } { applys* Forall_foreach_is_ge_inv Es. } }
-Qed.
-
-
-(* ********************************************************************** *)
-(* ********************************************************************** *)
-(* ********************************************************************** *)
-(** * Representation and lemmas *)
-
-
-(* ******************************************************* *)
-(** ** Data structure and definitions *)
-
-(** Functional representation of a node in a (nonempty) pairing heap *)
-
-Inductive node : Type :=
-  | Node : elem -> list node -> node.
-
-Instance Inhab_node : Inhab node.
-Proof using. applys Inhab_of_val (Node arbitrary nil). Qed.
-
-(** Functional representation of a possibly-empty pairing heap *)
-
-Definition heap := option node.
-
-Instance Inhab_heap : Inhab heap.
-Proof using. applys Inhab_of_val (@None node). Qed.
-
-(** [inv n E] relates a tree node [n] with the multiset [E] made of
-    the items that the tree contains *)
-
-Inductive inv : node -> elems -> Prop :=
-  | inv_Node : forall x ns Es E,
-      Forall2 inv ns Es ->
-      Forall (foreach (is_ge x)) Es ->
-      E = \{x} \u (list_union Es) ->
-      inv (Node x ns) E.
-
-
-(* ******************************************************* *)
-(** ** Lemmas and tactics *)
-
-(** An induction principle for trees -- should be automatically generated *)
-
-Section Node_induct.
-Variables
-(P : node -> Prop)
-(Q : list node -> Prop)
-(P2 : forall x l, Q l -> P (Node x l))
-(Q1 : Q nil)
-(Q2 : forall t l, P t -> Q l -> Q (t::l)).
-
-Fixpoint node_induct_gen (n : node) : P n :=
-  match n as x return P x with
-  | Node x l => P2 x
-      ((fix node_list_induct (l : list node) : Q l :=
-      match l as x return Q x with
-      | nil   => Q1
-      | t::l' => Q2 (node_induct_gen t) (node_list_induct l')
-      end) l)
-  end.
-
-End Node_induct.
-
-Lemma node_induct : forall (P : node -> Prop),
-  (forall (x : int) (l : list node),
-    (forall n, mem n l -> P n) -> P (Node x l)) ->
-  forall n : node, P n.
-Proof using.
-  introv Hn. eapply node_induct_gen with (Q := fun l =>
-    forall t, mem t l -> P t); intros.
-  auto. auto. inversions H. inversions~ H1.
-Qed.
-
-(** Implicit Types *)
-
-Implicit Types n : node.
-Implicit Types p q l : loc.
-Implicit Types x y : elem.
-Implicit Types h : heap.
-Implicit Types hs : list node.
-Implicit Types E : elems.
-Implicit Types Es : list elems.
-
-(** Key auxiliary lemmas for the verification proofs
-    (both for the functional version and the imperative version) *)
-
-Lemma inv_not_empty : forall n E,
-  inv n E ->
-  E <> \{}.
-Proof using. introv I. inverts I. multiset_inv. Qed.
-
-Lemma merge_lemma : forall x1 x2 ns1 ns2 Es1 Es2,
-  Forall2 inv ns1 Es1 ->
-  Forall2 inv ns2 Es2 ->
-  Forall (foreach (is_ge x2)) Es1 ->
-  Forall (foreach (is_ge x1)) Es2 ->
-  x1 <= x2 ->
-  inv (Node x1 (Node x2 ns1 :: ns2)) ('{x1} \u '{x2} \u list_union Es1 \u list_union Es2).
-Proof using.
-  introv Is1 Is2 Ks1 Ks2 L. applys_eq inv_Node. constructor.
-  { applys* inv_Node. }
-  { eauto. }
-  { constructors.
-    { applys foreach_union.
-      { applys* foreach_single. }
-      { applys* foreach_list_union. applys Forall_pred_incl Ks1.
-        { intros x Hx. applys* foreach_weaken. { intros y Hy. unfolds* is_ge. } } } }
-    { eauto. } }
-  { autos*. }
-Qed.
-
-
-
-(* ********************************************************************** *)
-(* ********************************************************************** *)
-(* ********************************************************************** *)
-(** * Imperative pairing heaps *)
-
-(* ******************************************************* *)
-(** ** Representation predicates *)
-
-(** [q ~> Tree n] is a notation for [Tree n q]. It relates a pointer [q] with the
-    functional tree structure [n] that it represents in memory *)
-
-Fixpoint Tree (n:node) (q:loc) { struct n } : hprop :=
-  match n with
-  | Node x hs =>
-      \exists (q':loc),
-         q  ~~~>`{ value' := x; child' := q' }
-      \* q' ~> MListOf Tree hs
-  end.
-
-(** [q ~> Repr E] related a pointer [q] with the multiset of items [E]
-    that are stored in the tree *)
-
-Definition Repr (E:elems) (q:loc) : hprop :=
-  \exists n, q ~> Tree n \* \[inv n E].
-
-(** [q ~> Heap E] relates a pointer on a heap [p] with the multiset of items [E]
-    that are stored in the heap. It uses [Contents E c] as an auxiliary definition. *)
-
-Definition Contents (E:elems) (c:contents_) : hprop :=
-  match c with
-  | Empty => \[E = \{}]
-  | Nonempty p => (p ~> Repr E)
-  end.
-
-Definition Heap (E:elems) (p:heap_) : hprop :=
-  \exists c, p ~~> c \* Contents E c.
-
-
-(* ******************************************************* *)
-(** ** Paraphrase definitions as equalities *)
-
-Lemma Tree_Node : forall q x hs,
-  q ~> Tree (Node x hs) =
-      \exists l, q ~~~> `{ value' := x; child' := l }
-              \* l ~> MListOf Tree hs.
-Proof using. auto. Qed.
-
-Lemma Contents_eq : forall E c,
-  Contents E c = (match c with
-  | Empty => \[E = \{}]
-  | Nonempty p => (p ~> Repr E)
-  end).
-Proof using. auto. Qed.
-
-Lemma Heap_eq : forall p E,
-  p ~> Heap E = \exists c, p ~~> c \* Contents E c.
-Proof using. auto. Qed.
-
-Lemma Repr_eq : forall q E,
-  q ~> Repr E = \exists n, q ~> Tree n \* \[inv n E].
-Proof using. auto. Qed.
-
-Lemma haffine_Tree : forall n p,
-  haffine (p ~> Tree n).
-Proof using.
-  intros n. induction n using node_induct.
-  intros. xunfold Tree. xaffine.
-Qed.
-
-Hint Resolve haffine_Tree : haffine.
-
-
-(* ******************************************************* *)
-(** ** Lemmas about representation predicates *)
-
-Lemma Repr_not_empty : forall q E,
-  q ~> Repr E ==> \[E <> \{}] \* q ~> Repr E.
-Proof using.
-  intros. xunfold Repr. xpull ;=> n I. lets: inv_not_empty I. xsimpl*.
-Qed.
-
-Lemma Contents_is_empty : forall c E,
-  Contents E c ==> \[c = Empty <-> E = \{}] \* Contents E c.
-Proof using.
-  intros.  unfold Contents. destruct c.
-  { xsimpl*. }
-  { xchange Repr_not_empty ;=> N. xsimpl. iff H; false. }
-Qed.
-
-Lemma Heap_Nonempty : forall p q E,
-  p ~~> Nonempty q \* q ~> Repr E ==> p ~> Heap E.
-Proof using.
-  intros. xchanges Repr_not_empty ;=> N. xunfold Heap. xsimpl.
-Qed.
-
-Lemma Heap_Empty : forall p,
-  p ~~> Empty ==> p ~> Heap \{}.
-Proof using. intros. xunfold Heap. unfold Contents. xsimpl*. Qed.
-
-
-(* ******************************************************* *)
-(** ** Verification *)
-
-Lemma Triple_create :
-  SPEC (create tt)
-    PRE \[]
-    POST (fun p => p ~> Heap \{}).
-Proof using.
-  xcf. xapp. xunfold Heap. unfold Contents. xsimpl*.
-Qed.
-
-Hint Extern 1 (RegisterSpec create) => Provide Triple_create.
-
-Lemma Triple_is_empty : forall p E,
-  SPEC (is_empty p)
-    PRE (p ~> Heap E)
-    POST (fun b => \[b = isTrue (E = \{})] \* p ~> Heap E).
-Proof using.
-  xcf. xunfolds Heap ;=> q. xapp. xapp.
-  xchanges~ Contents_is_empty.
-Qed.
-
-Hint Extern 1 (RegisterSpec (is_empty)) => Provide Triple_is_empty.
-
-Lemma Triple_merge : forall q1 q2 E1 E2,
-  SPEC (merge q1 q2)
-    PRE (q1 ~> Repr E1 \* q2 ~> Repr E2)
-    POST (fun q => q ~> Repr (E1 \u E2)).
-Proof using.
-  xcf. xchange (Repr_eq q1) ;=> [x1 hs1] I1.
-  xchange (Repr_eq q2) ;=> [x2 hs2] I2.
-  xchange (Tree_Node q1) ;=> l1.
-  xchange (Tree_Node q2) ;=> l2.
-  inverts I1 as Is1 Ks1. inverts I2 as Is2 Ks2.
-  xapp. 
-  xif ;=> C.
-  { xapp. xchange <- (Tree_Node q2). xapp.
-    xchange <- Tree_Node. xchange <- Repr_eq.
-    applys* merge_lemma. xvals*. }
-  { xapp. xchange <- (Tree_Node q1). xapp.
-    xchange <- Tree_Node. xchange <- Repr_eq.
-    applys* merge_lemma. xvals*. }
-Qed.
-
-Hint Extern 1 (RegisterSpec merge) => Provide Triple_merge.
-
-Lemma Triple_insert : forall p x E,
-  SPEC (insert p x)
-    PRE (p ~> Heap E)
-    POST (fun (_:unit) => p ~> Heap (E \u \{x})).
-Proof using.
-  xcf. xchange Heap_eq ;=> q. xapp ;=> l. xapp ;=> q2.
-  xchange <- Tree_Node. xchange <- Repr_eq. { applys* inv_Node. }
-  rew_listx. xapp. xmatch; simpl.
-  { xpull ;=> ->. xapp. xchanges* Heap_Nonempty. }
-  { xapp ;=> r. xapp. xchanges* Heap_Nonempty. }
-Qed.
-
-Hint Extern 1 (RegisterSpec insert) => Provide Triple_insert.
-
-Lemma Triple_merge_pairs : forall ns l Es,
-  ns <> nil ->
-  Forall2 inv ns Es ->
-  SPEC (merge_pairs l)
-    PRE (l ~> MListOf Tree ns)
-    POST (fun q => q ~> Repr (list_union Es)).
-Proof using.
-  intros ns. induction_wf IH: list_sub ns; introv N Is.
-  xcf. xapp~ ;=> q1 n1 ns' ->. inverts Is as I1 Is. rename r into Es'.
-  xif ;=> C.
-  { subst. inverts Is. rew_listx. xval. xchanges* <- Repr_eq. }
-  { xapp~ ;=> q2 n2 ns'' ->. inverts Is as I2 Is. rename r into Es''.
-    do 2 xchange* <- Repr_eq. xapp ;=> r. xif ;=> C'.
-    { subst. inverts Is. rew_listx. xval. xsimpl. }
-    { xapp* ;=> r'. xapp ;=> r''. rew_listx. xsimpl*. } }
-Qed.
-
-Hint Extern 1 (RegisterSpec merge_pairs) => Provide Triple_merge_pairs.
-
-Lemma Triple_pop_min : forall p E,
-  E <> \{} ->
-  SPEC (pop_min p)
-    PRE (p ~> Heap E)
-    POST (fun x => \exists E', \[min_of E x /\ E = \{x} \u E'] \* p ~> Heap E').
-Proof using.
-  introv HE. xcf. xchange Heap_eq ;=> c. xapp.
-  destruct c as [|q]; simpl; xpull.
-  xchange Repr_eq ;=> [x hs] I. invert I ;=> ? ? ? ? Is Ks Eq -> -> ->.
-  xchange Tree_Node ;=> l. xmatch. xapp. xapp. xapp.
-  xseq (fun (_:unit) => \exists E', \[E = '{x} \u E'] \* p ~> Heap E' \* \GC).
-  { xif ;=> C2.
-    { subst. inverts Is. inverts Ks. rew_listx. xapp. xchanges* Heap_Empty. }
-    { xapp. xapp* ;=> r. xapp. xchange Heap_Nonempty. xsimpl*. } }
-  { xpull ;=> E' ->. xval. xsimpl. split~. { rewrite Eq. applys~ pop_min_lemma. } }
-Qed.
-
-Hint Extern 1 (RegisterSpec pop_min) => Provide Triple_pop_min.
